Cslib/Computability/Machines/MultiTapeTuring/PopRoutine.lean
@@ -53,7 +53,7 @@ public def pop' {k aux : ℕ} (i : ℕ) (h_i_lt : i < k := by decide) :
 public theorem pop'_eval_list {k aux i : ℕ} {h_i_lt : i < k}
   {tapes : Fin k → List (List α)}
   {h_not_empty : tapes ⟨i, h_i_lt⟩ ≠ []} :
-  (pop' (aux := aux) i h_i_lt).eval_list tapes = .some
+  (pop' (aux := aux) i h_i_lt).eval_list_aux tapes = .some
     (Function.update tapes ⟨i, h_i_lt⟩ (tapes ⟨i, h_i_lt⟩).tail) := by
   sorry
 
